isabelle/CVM_Subsample/CVM_New_Unbiased_Algorithm.thy
@@ -52,84 +52,80 @@ begin
 unbundle no_vec_syntax
 
 context
-  fixes subsample_size :: nat
-  fixes thresh :: nat
-  assumes subsample_size: \<open>subsample_size < thresh\<close> \<open>2 * subsample_size \<ge> thresh\<close>
+  fixes f :: real and n :: nat
+  assumes f_range: \<open>f \<in> {1/2..<1}\<close> \<open>n * f \<in> \<nat>\<close> and n_gt_0: \<open>n > 0\<close>
 begin
 
-text \<open>Line 1:\<close>
-definition initial_state :: \<open>'a state\<close> where
-  \<open>initial_state \<equiv> \<lparr>state_p = 1, state_\<chi> = {}\<rparr>\<close>
+definition \<open>initial_state = State {} 1\<close> \<comment> \<open>Setup initial state $\chi=\emptyset$ and $p=1$.\;\<close>
+definition subsample where
+  \<open>subsample \<chi> = pmf_of_set {S. S \<subseteq> \<chi> \<and> card S = n * f}\<close> \<comment> \<open>Sample random $n f$ subset.\;\<close>
 
-definition f :: real
-  where \<open>f \<equiv> subsample_size / thresh\<close>
+fun step where \<comment> \<open>Loop body.\;\<close>
+  \<open>step a (State \<chi> p) = do {
+    b \<leftarrow> bernoulli_pmf p;
+    let \<chi> = (if b then \<chi> \<union> {a} else \<chi> - {a});
 
-text \<open>Lines 3--7:\<close>
-definition step_1 :: \<open>'a \<Rightarrow> 'a state \<Rightarrow> 'a state pmf\<close> where
-  \<open>step_1 x \<sigma> =
-    do {
-      let p = state_p \<sigma>;
-      let \<chi> = state_\<chi> \<sigma>;
-
-      insert_x_into_\<chi> \<leftarrow> bernoulli_pmf p;
-
-      let \<chi> = (
-        if insert_x_into_\<chi>
-        then insert x \<chi>
-        else Set.remove x \<chi>
-      );
-
-      return_pmf (\<sigma>\<lparr>state_\<chi> := \<chi>\<rparr>)
-    }\<close>
-
-definition subsample :: \<open>'a set \<Rightarrow> 'a set pmf\<close> where
-  \<open>subsample \<chi> = pmf_of_set {S. S \<subseteq> \<chi> \<and> card S = subsample_size}\<close>
-
-text \<open>Lines 8--10:\<close>
-definition step_2 :: \<open>'a state \<Rightarrow> 'a state pmf\<close> where
-  \<open>step_2 \<sigma> = do {
-    let p = state_p \<sigma>;
-    let \<chi> = state_\<chi> \<sigma>;
-
-    if card \<chi> = thresh
-    then do {
+    if card \<chi> = n then do {
       \<chi> \<leftarrow> subsample \<chi>;
-      return_pmf \<lparr>state_p = p * f, state_\<chi> = \<chi>\<rparr>
-    } else
-      return_pmf \<sigma>
-    }\<close>
+      return_pmf (State \<chi> (p * f))
+    } else do {
+      return_pmf (State \<chi> p)
+    }
+   }\<close>
 
-text \<open>Lines 1--10:\<close>
-definition run_steps :: \<open>'a list \<Rightarrow> 'a state pmf\<close> where
-  \<open>run_steps xs \<equiv> foldM_pmf (\<lambda>x \<sigma>. step_1 x \<sigma> \<bind> step_2) xs initial_state\<close>
+definition \<open>run_steps xs = foldM_pmf step xs initial_state\<close> \<comment> \<open>Iterate loop over stream @{term xs}.\;\<close>
+definition \<open>estimate \<sigma> = card (state_\<chi> \<sigma>) / state_p \<sigma>\<close>
+definition \<open>run_algo xs = map_pmf estimate (run_steps xs)\<close> \<comment> \<open>Run algorithm and estimate.\;\<close>
 
-text \<open>Line 11:\<close>
-definition estimate :: \<open>'a state \<Rightarrow> real\<close> where
-  \<open>estimate \<sigma> = card (state_\<chi> \<sigma>) / state_p \<sigma>\<close>
+definition \<open>subsample_size = (THE x. real x = n * f)\<close>
 
-definition run_algo :: \<open>'a list \<Rightarrow> real pmf\<close> where
-  \<open>run_algo xs = map_pmf estimate (run_steps xs)\<close>
+lemma subsample_size_eq:
+  \<open>real subsample_size = n * f\<close>
+proof -
+  obtain a where a_def:\<open>real a = real n * f\<close> using f_range(2) by (metis Nats_cases)
+  show ?thesis
+    unfolding subsample_size_def using a_def
+    by (rule theI2[where a=\<open>a\<close>]) (use a_def in auto)
+qed
+
+lemma subsample_size:
+  \<open>subsample_size < n\<close> \<open>2 * subsample_size \<ge> n\<close>
+proof (goal_cases)
+  case 1
+  have \<open>real subsample_size < real n\<close>
+    unfolding subsample_size_eq using f_range(1) n_gt_0 by auto
+  thus ?case by simp
+next
+  case 2
+  have \<open>real n \<le> 2 * real subsample_size\<close>
+    using f_range(1) n_gt_0 unfolding subsample_size_eq by auto
+  thus ?case by simp
+qed
 
 lemma subsample_finite_nonempty:
-  assumes \<open>card U = thresh\<close>
+  assumes \<open>card U = n\<close>
   shows
     \<open>{T. T \<subseteq> U \<and> card T = subsample_size} \<noteq> {}\<close> (is \<open>?C \<noteq> {}\<close>)
     \<open>finite {T. T \<subseteq> U \<and> card T = subsample_size}\<close>
+    \<open>subsample U = pmf_of_set {T. T \<subseteq> U \<and> card T = subsample_size}\<close>
     \<open>finite (set_pmf (subsample U))\<close>
 proof -
   have fin_U: \<open>finite U\<close> using assms subsample_size
     by (meson card_gt_0_iff le0 order_le_less_trans order_less_le_trans)
   have a: \<open>card U choose subsample_size > 0\<close>
     using subsample_size assms by (intro zero_less_binomial) auto
+  show b:\<open>subsample U = pmf_of_set ?C\<close>
+    using subsample_size_eq
+    unfolding subsample_def by (intro arg_cong[where f=\<open>pmf_of_set\<close>] Collect_cong) auto
   with assms subsample_size have \<open>card ?C > 0\<close>
     using n_subsets[OF fin_U] by simp
   thus \<open>?C \<noteq> {}\<close> \<open>finite ?C\<close> using card_gt_0_iff by blast+
-  thus \<open>finite (set_pmf (subsample U))\<close> unfolding subsample_def by auto
+  thus \<open>finite (set_pmf (subsample U))\<close> unfolding b by auto
 qed
 
 lemma int_prod_subsample_eq_prod_int:
   fixes g :: \<open>bool \<Rightarrow> real\<close>
-  assumes \<open>card U = thresh\<close> \<open>S \<subseteq> U\<close> \<open>range g \<subseteq> {0..}\<close>
+  assumes \<open>card U = n\<close> \<open>S \<subseteq> U\<close> \<open>range g \<subseteq> {0..}\<close>
   shows \<open>(\<integral>\<omega>. (\<Prod>s\<in>S. g(s \<in> \<omega>)) \<partial>subsample U) \<le> (\<Prod>s\<in>S. (\<integral>\<omega>. g \<omega> \<partial>bernoulli_pmf f))\<close> (is \<open>?L \<le> ?R\<close>)
 proof -
   define \<eta> where \<open>\<eta> \<equiv> if g True \<ge> g False then Fwd else Rev\<close>
@@ -137,10 +133,9 @@ proof -
   have fin_U: \<open>finite U\<close> using assms subsample_size
     by (meson card_gt_0_iff le0 order_le_less_trans order_less_le_trans)
 
-  note subsample_finite_nonempty =
-    subsample_finite_nonempty[OF assms(1)]
+  note subsample = subsample_finite_nonempty[OF assms(1)]
 
-  note [simp] = integrable_measure_pmf_finite[OF subsample_finite_nonempty(3)]
+  note [simp] = integrable_measure_pmf_finite[OF subsample(4)]
 
   let ?C = \<open>{T. T \<subseteq> U \<and> card T = subsample_size}\<close>
 
@@ -148,7 +143,7 @@ proof -
     using subsample_size unfolding assms(1) by simp
 
   have \<open>measure_pmf.neg_assoc (subsample U) (\<lambda>s \<omega>. (s \<in> \<omega>)) U\<close>
-    using subssample_size_le_card_U unfolding subsample_def
+    using subssample_size_le_card_U unfolding subsample
     by (intro n_subsets_distribution_neg_assoc fin_U)
 
   hence na: \<open>measure_pmf.neg_assoc (subsample U) (\<lambda>s \<omega>. (s \<in> \<omega>)) S\<close>
@@ -167,9 +162,9 @@ proof -
   proof -
     have \<open>measure (pmf_of_set ?C) {x. s \<in> x} = real subsample_size / card U\<close>
       by (intro n_subsets_prob subssample_size_le_card_U that fin_U)
-    also have \<open>\<dots> = f\<close> unfolding f_def assms(1) by simp
+    also have \<open>\<dots> = f\<close> unfolding subsample_size_eq  assms(1) using n_gt_0 by auto
     finally have \<open>measure (pmf_of_set ?C) {x. s \<in> x} = f\<close> by simp
-    thus ?thesis by (intro eq_bernoulli_pmfI) (simp add: pmf_map vimage_def subsample_def)
+    thus ?thesis by (intro eq_bernoulli_pmfI) (simp add: pmf_map vimage_def subsample)
   qed
 
   have \<open>?L \<le> (\<Prod>s\<in>S. (\<integral>\<omega>. g (s \<in> \<omega>) \<partial>subsample U))\<close>
@@ -179,56 +174,56 @@ proof -
   finally show ?thesis .
 qed
 
-interpretation abs: cvm_algo_abstract thresh f subsample
+schematic_goal step_n_def: \<open>step x \<sigma> = ?x\<close>
+  by (subst state.collapse[symmetric], subst step.simps, rule refl)
+
+interpretation abs: cvm_algo_abstract n f subsample
   rewrites \<open>abs.run_steps = run_steps\<close> and \<open>abs.estimate = estimate\<close>
 proof -
-  show abs:\<open>cvm_algo_abstract thresh f subsample\<close>
+  show abs:\<open>cvm_algo_abstract n f subsample\<close>
   proof (unfold_locales, goal_cases)
     case 1 thus ?case using subsample_size by auto
   next
-    case 2 thus ?case using subsample_size unfolding f_def by auto
+    case 2 thus ?case using f_range by auto
   next
-    case (3 U x) thus ?case using subsample_finite_nonempty[OF 3(1)] unfolding subsample_def by simp
+    case (3 U x) thus ?case using subsample_finite_nonempty[OF 3(1)] by simp
   next
     case (4 g U S) thus ?case by (intro int_prod_subsample_eq_prod_int) auto
   qed
-  have a:\<open>cvm_algo_abstract.step_1 = step_1\<close>
-    unfolding cvm_algo_abstract.step_1_def[OF abs] step_1_def by auto
-  have b:\<open>cvm_algo_abstract.step_2 thresh f subsample = step_2\<close>
-    unfolding cvm_algo_abstract.step_2_def[OF abs] step_2_def Let_def by (auto simp:map_pmf_def)
+  have a:\<open>(\<lambda>x \<sigma>. cvm_algo_abstract.step_1 x \<sigma> \<bind> cvm_algo_abstract.step_2 n f subsample) = step\<close>
+    unfolding cvm_algo_abstract.step_1_def[OF abs]  cvm_algo_abstract.step_2_def[OF abs] step_n_def
+    by (intro ext) (simp add: bind_assoc_pmf Let_def bind_return_pmf Set.remove_def cong:if_cong)
   have c:\<open>cvm_algo_abstract.initial_state = initial_state\<close>
     unfolding cvm_algo_abstract.initial_state_def[OF abs] initial_state_def by auto
-  show \<open>cvm_algo_abstract.run_steps thresh f subsample = run_steps\<close>
-    unfolding cvm_algo_abstract.run_steps_def[OF abs] run_steps_def a b c by simp
+  show \<open>cvm_algo_abstract.run_steps n f subsample = run_steps\<close>
+    unfolding cvm_algo_abstract.run_steps_def[OF abs] run_steps_def a c by simp
   show \<open>cvm_algo_abstract.estimate = estimate\<close>
     unfolding cvm_algo_abstract.estimate_def[OF abs] estimate_def by auto
 qed
 
-theorem unbiasedness:
-  \<open>measure_pmf.expectation (run_steps xs) estimate = card (set xs)\<close>
-  by (rule abs.unbiasedness)
+theorem unbiasedness: \<open>measure_pmf.expectation (run_algo xs) id = card (set xs)\<close>
+  unfolding run_algo_def integral_map_pmf using abs.unbiasedness by simp
 
 theorem correctness:
-  fixes \<epsilon> \<delta> :: real
-  assumes \<open>\<epsilon> \<in> {0<..<1}\<close> \<open>\<delta> \<in> {0<..<1}\<close>
-  assumes \<open>real thresh \<ge> 12 / \<epsilon> ^ 2 * ln (3 * real (length xs) / \<delta>)\<close>
+  assumes \<open>\<epsilon> \<in> {0<..<1::real}\<close> \<open>\<delta> \<in> {0<..<1::real}\<close>
+  assumes \<open>real n \<ge> 12 / \<epsilon>\<^sup>2 * ln (3 * real (length xs) / \<delta>)\<close>
   defines \<open>A \<equiv> real (card (set xs))\<close>
-  shows \<open>\<P>(\<sigma> in run_algo xs. \<bar>\<sigma> - A\<bar> > \<epsilon> * A) \<le> \<delta>\<close>
+  shows \<open>\<P>(R in run_algo xs. \<bar>R - A\<bar> > \<epsilon> * A) \<le> \<delta>\<close>
   using assms(3) unfolding A_def run_algo_def using abs.correctness[OF assms(1,2)] by auto
 
 lemma space_usage:
-  \<open>AE \<sigma> in run_steps xs. card (state_\<chi> \<sigma>) < thresh \<and> finite (state_\<chi> \<sigma>)\<close>
+  \<open>AE \<sigma> in run_steps xs. card (state_\<chi> \<sigma>) < n \<and> finite (state_\<chi> \<sigma>)\<close>
 proof -
   define \<rho> where \<open>\<rho> = FinalState xs\<close>
-  have \<open>card (state_\<chi> \<sigma>) < thresh + (case \<rho> of FinalState _ \<Rightarrow> 0 | IntermState _ _ \<Rightarrow> 1)\<close>
+  have \<open>card (state_\<chi> \<sigma>) < n + (case \<rho> of FinalState _ \<Rightarrow> 0 | IntermState _ _ \<Rightarrow> 1)\<close>
     if \<open>\<sigma> \<in> set_pmf (abs.run_state_pmf \<rho>)\<close> for \<sigma>
     using that
   proof (induction \<rho> arbitrary:\<sigma> rule:run_state_induct)
     case 1
-    then show ?case using abs.thresh_gt_0 by (simp add:run_steps_def initial_state_def)
+    then show ?case using n_gt_0 by (simp add:run_steps_def initial_state_def)
   next
     case (2 xs x)
-    have \<open>card (state_\<chi> \<tau>) < thresh \<and> finite (state_\<chi> \<tau>)\<close>
+    have \<open>card (state_\<chi> \<tau>) < n \<and> finite (state_\<chi> \<tau>)\<close>
       if \<open>\<tau> \<in> set_pmf (abs.run_state_pmf (FinalState xs))\<close> for \<tau>
       using 2(1) abs.state_\<chi>_finite[where \<rho>=\<open>FinalState xs\<close>] that by (simp add:AE_measure_pmf_iff)
     thus ?case
@@ -242,22 +237,22 @@ proof -
       by (simp add:p_def abs.run_steps_snoc)
 
     have b:\<open>card \<chi> < card (state_\<chi> \<tau>)\<close>
-      if \<open>card (state_\<chi> \<tau>) = thresh\<close> \<open>\<chi> \<in> set_pmf (subsample (state_\<chi> \<tau>))\<close> \<open>\<tau> \<in> set_pmf p\<close> for \<chi> \<tau>
+      if \<open>card (state_\<chi> \<tau>) = n\<close> \<open>\<chi> \<in> set_pmf (subsample (state_\<chi> \<tau>))\<close> \<open>\<tau> \<in> set_pmf p\<close> for \<chi> \<tau>
     proof -
       from subsample_finite_nonempty[OF that(1)]
       have \<open>card \<chi> = subsample_size\<close> using that unfolding subsample_def by auto
       thus ?thesis using subsample_size(1) that by auto
     qed
 
-    have \<open>card (state_\<chi> \<tau>) < thresh \<or> card (state_\<chi> \<tau>) = thresh\<close> \<open>finite (state_\<chi> \<tau>)\<close>
+    have \<open>card (state_\<chi> \<tau>) < n \<or> card (state_\<chi> \<tau>) = n\<close> \<open>finite (state_\<chi> \<tau>)\<close>
       if \<open>\<tau> \<in> set_pmf p\<close> for \<tau>
       using 3(1) abs.state_\<chi>_finite[where \<rho>=\<open>IntermState xs x\<close>] that unfolding p_def
       by (auto simp:AE_measure_pmf_iff less_Suc_eq)
-    hence \<open>card (state_\<chi> \<sigma>) < thresh\<close>
+    hence \<open>card (state_\<chi> \<sigma>) < n\<close>
       using 3(2) unfolding a abs.step_2_def Let_def by (auto intro!:b simp:if_distrib if_distribR)
     thus ?case by simp
   qed
-  thus ?thesis using abs.state_\<chi>_finite[where \<rho>=\<open>FinalState xs\<close>]  unfolding \<rho>_def
+  thus ?thesis using abs.state_\<chi>_finite[where \<rho>=\<open>FinalState xs\<close>] unfolding \<rho>_def
     by (simp add:AE_measure_pmf_iff)
 qed
 
